-restructured problems in complexity -added the TM-problems we will use

theories/L/Complexity/Problems/TMGenNP_fixed_mTM.v
@@ -9,17 +9,22 @@ From Undecidability Require Import L.Datatypes.LNat.
 (** For each Machine M (with n+1 tapes), we define this problem:
 Given n tapes and a sizeBound and a step bound, does there exist a (small enough) first tape such that the machine halts on the resulting n+1 tapes in fewer? *)
 
-Definition TMGenNP_fixed_mTM' (sig : finType) `{registered sig} n (M : mTM sig (S n)) : Vector.t (tape sig) n * nat * nat -> Prop :=
-  fun '(ts, maxSize, steps) =>
-    exists t1, sizeOfTape t1 <= maxSize /\ exists f, loopM (initc M (t1:::ts)) steps = Some f.
-
+(** We contain this on haltsOrDiverges as out MutiTape2SingleTape-translation probably only knows upper bounds of the step count.  *)
 Definition HaltsOrDiverges_fixed_mTM (sig : finType) `{registered sig} n (M : mTM sig (S n)) : Vector.t (tape sig) n * nat * nat -> Prop :=
   fun '(ts, maxSize, steps) =>
     forall t1, sizeOfTape t1 <= maxSize -> forall k f, loopM (initc M (t1:::ts)) steps = Some f -> k <= steps.
 
 Definition TMGenNP_fixed_mTM (sig : finType) `{registered sig} n (M : mTM sig (S n))
-  := restrictBy (HaltsOrDiverges_fixed_mTM M) (TMGenNP_fixed_mTM' M).
+  := (fun '(ts, maxSize, steps) =>
+        exists t1, sizeOfTape t1 <= maxSize /\ exists f, loopM (initc M (t1:::ts)) steps = Some f).
 
 Arguments TMGenNP_fixed_mTM : clear implicits.
 Arguments TMGenNP_fixed_mTM {_ _ _}.
 
+
+Definition TMGenNP_fixed_singleTapeTM (sig : finType) `{registered sig} (M : mTM sig 1)
+  := (fun '(ts, maxSize, steps) =>
+        exists s1 (t1 : list sig), length t1 <= maxSize /\ exists f, loopM (initc M [|leftof s1 (t1++ts)|] ) steps = Some f).
+
+Arguments TMGenNP_fixed_singleTapeTM : clear implicits.
+Arguments TMGenNP_fixed_singleTapeTM {_ _}.
