theories/L/Complexity/Reductions/TMGenNP/mTM_to_singleTapeTM.v
@@ -1,0 +1,18 @@
+From Undecidability.L Require Import Tactics.LTactics.
+From Undecidability.L.Datatypes Require Import Lists LVector.
+From Undecidability.L.Complexity Require Import NP Synthetic Monotonic.
+From Undecidability.TM Require Import TM Single.StepTM.
+
+From Undecidability.L.Complexity  Require GenNP.
+From Undecidability.L.Complexity  Require Import LMGenNP TMGenNP_fixed_mTM.
+
+
+From Undecidability Require Import TM.Single.EncodeTapes.
+
+
+Lemma LMGenNP_to_TMGenNP_mTM (sig:finType) (n:nat) `{R__sig : registered sig}  (M : mTM sig (S n)):
+  exists sig' `{R__sig' : registered sig'} (M' : mTM sig 1),
+    restrictBy (HaltsOrDiverges_fixed_mTM M) (TMGenNP_fixed_mTM M)
+               ⪯p unrestrictedP (TMGenNP_fixed_singleTapeTM M').
+Proof.
+Abort.
